checkpoint, before simplifying frame condition on actions

pulse/lib/pulse_core/Pulse.MonotonicStateMonad.fst
@@ -1,8 +1,6 @@
 module Pulse.MonotonicStateMonad
 open FStar.Preorder
-
-#push-options "--print_universes"
-
+module M = FStar.MSTTotal
 let mst (#s:Type u#s)
          (rel:FStar.Preorder.preorder s)
          (a:Type u#a)
@@ -15,6 +13,25 @@ let mst (#s:Type u#s)
             rel s0 res._2
         }
     )
+
+assume
+val reify_ (#s:Type u#2) (#rel:FStar.Preorder.preorder s)
+           (#a:Type u#a) (#pre:s -> prop) (#post:s -> a -> s -> prop)
+           ($f:unit -> M.MSTATETOT a s rel pre post)
+: M.repr a s rel pre post
+
+let of_msttotal (#s:Type u#2) (rel:FStar.Preorder.preorder s)
+                (a:Type u#a) (pre:s -> prop) (post:s -> a -> s -> prop)
+                (f:unit -> M.MSTATETOT a s rel pre post)
+: mst rel a pre post
+= let f = reify_ f in
+  fun s -> f s
+
+let to_msttotal (#s:Type u#2) (rel:FStar.Preorder.preorder s)
+                (a:Type u#a) (pre:s -> prop) (post:s -> a -> s -> prop)
+                (f:mst rel a pre post)
+: M.MSTATETOT a s rel pre post
+= M.MSTATETOT?.reflect (fun s -> f s)
 
 let return x
 = fun s0 -> x, s0
