pulse/lib/pulse_core/PulseCore.InstantiatedSemantics.fst
@@ -1,65 +1,67 @@
 module PulseCore.InstantiatedSemantics
 module Sem = PulseCore.Semantics2
 module Mem = PulseCore.Memory
+open Mem
 
 let laws ()
 : squash (
-    Sem.associative Mem.star /\
-    Sem.commutative Mem.star /\
-    Sem.is_unit Mem.emp Mem.star
+    Sem.associative star /\
+    Sem.commutative star /\
+    Sem.is_unit emp star
   )
-= let open Mem in
-  let equiv_eq (x y:slprop)
+= let equiv_eq (x y:slprop)
     : Lemma (x `equiv` y <==> x == y)
           [SMTPat (x `equiv` y)]
     = introduce x `equiv` y ==> x == y
-      with _h . Mem.slprop_extensionality x y
+      with _h . slprop_extensionality x y
   in
   let _ : squash (Sem.associative star) =
     introduce 
         forall x y z. 
             ((x `star` y) `star` z) ==
             (x `star` (y `star` z))
-    with Mem.star_associative x y z
+    with star_associative x y z
   in
   let _ : squash (Sem.commutative star) = 
     introduce 
         forall x y.
             x `star` y == y `star` x
-        with Mem.star_commutative x y
+        with star_commutative x y
   in
   let _ : squash (Sem.is_unit emp star) =
     introduce
         forall x.
             (x `star` emp) == x /\
             (emp `star` x) == x
-        with Mem.emp_unit x
+        with emp_unit x
   in
   ()
 
-let state : Sem.state = {
-    s = Mem.mem;
-    is_full_mem = Mem.full_mem_pred;
-    pred = Mem.slprop;
-    emp = Mem.emp;
-    star = Mem.star;
-    interp = Mem.interp;
-    evolves = Mem.mem_evolves;
-    invariant = Mem.locks_invariant Set.empty;
+let state0 (e:inames) : Sem.state = {
+    s = mem;
+    is_full_mem = full_mem_pred;
+    pred = slprop;
+    emp = emp;
+    star = star;
+    interp = interp;
+    evolves = mem_evolves;
+    invariant = locks_invariant e;
     laws = laws ()
 }
 
+let state : Sem.state = state0 Set.empty
+
+(* The type of general-purpose computations *)
 let stt (a:Type u#a) 
-        (pre:Mem.slprop)
-        (post:a -> Mem.slprop)
+        (pre:slprop)
+        (post:a -> slprop)
 : Type0
 = unit -> Dv (Sem.m u#2 u#a #state a pre post)
 
-let return (#a:Type u#a) (x:a) (p:a -> Mem.slprop)
+let return (#a:Type u#a) (x:a) (p:a -> slprop)
 : stt a (p x) p
 = fun _ -> Sem.ret x p
 
-open Mem
 let bind_stt
     (#a:Type u#a) (#b:Type u#b)
     (#pre1:slprop) (#post1:a -> slprop) (#post2:b -> slprop)
@@ -75,3 +77,94 @@ let frame_stt
   (e:stt a pre post)
 : stt a (pre `star` frame) (fun x -> post x `star` frame)
 = fun _ -> Sem.frame frame (e())
+
+(* The type of atomic actions *)
+module M = Pulse.MonotonicStateMonad
+let action
+    (a:Type u#a)
+    (except:inames)
+    (pre:slprop)
+    (post:a -> slprop)
+= frame:slprop ->
+  Sem.mst_sep_aux u#2 u#a state
+    (inames_ok except)
+    (state0 except).invariant
+    a 
+    (pre `star` frame)
+    (fun x -> post x `star` frame)
+
+let return_action
+    (#a:Type u#a)
+    (#except:inames)
+    (#post:a -> slprop)
+    (x:a)
+: action a except (post x) post
+= fun frame -> M.weaken (M.return x)
+
+let bind_action
+     (#a:Type u#a)
+     (#b:Type u#b)
+     (#except:inames)
+     (#pre1 #post1 #post2:_)
+     (f:action a except pre1 post1)
+     (g:(x:a -> action b except (post1 x) post2))
+: action b except pre1 post2
+= fun frame -> M.weaken (M.bind (f frame) (fun x -> g x frame))
+
+let frame_action
+     (#a:Type u#a)
+     (#b:Type u#b)
+     (#except:inames)
+     (#pre #post #frame:_)
+     (f:action a except pre post)
+: action a except (pre `star` frame) (fun x -> post x `star` frame)
+= fun frame' -> f (frame `star` frame')
+
+let stt_of_action (#a:Type u#2) #pre #post (m:action a Set.empty pre post)
+: stt a pre post
+= let step (frame:slprop)
+    : Sem.mst_sep state a (pre `star` frame) (fun x -> post x `star` frame)
+    = M.weaken (m frame)
+  in
+  let action : Sem.action state a = {pre=pre; post=post; step} in
+  let m : Sem.m a pre post = Sem.act action in
+  fun _ -> m
+
+module MST = Pulse.MonotonicStateMonad
+
+let mem_action_as_action
+        (a:Type u#a)
+        (except:inames)
+        (req:slprop)
+        (ens: a -> slprop)
+        (act:Mem.action_except a except req ens)
+: action a except req ens
+= fun frame ->
+    let thunk
+      : unit -> MstTot a except req ens frame (fun _ -> True) (fun _ _ _ -> True)
+      = fun _ -> act frame
+    in
+    MST.of_msttotal _ _ _ _ thunk
+
+let action_as_mem_action
+        (a:Type u#a)
+        (except:inames)
+        (pre:slprop)
+        (post: a -> slprop)
+        (act:action a except pre post)
+: Mem.action_except a except pre post
+= fun frame ->
+    let m
+      : MST.mst state.evolves
+                a 
+                (fun s0 -> 
+                    inames_ok except s0 /\
+                    interp ((pre `star` locks_invariant except s0) `star` frame) s0)
+                (fun s0 x s1 ->
+                    inames_ok except s1 /\
+                    interp ((post x `star` locks_invariant except s1) `star` frame) s1 /\
+                    (forall (f_frame:mprop frame). f_frame (core_mem s0) == f_frame (core_mem s1)))
+      = magic() //MST.weaken (act frame)
+    in
+    MST.to_msttotal _ _ _ _ m
+    // MST.to_msttotal _ _ _ _ m
