pulse/lib/pulse_core/Pulse.NondeterministicMonotonicStateMonad.fsti
@@ -1,6 +1,7 @@
 module Pulse.NondeterministicMonotonicStateMonad
 open FStar.Preorder
-
+open Pulse.MonotonicStateMonad
+module M = Pulse.MonotonicStateMonad
 
 val nmst (#s:Type u#s)
          (rel:FStar.Preorder.preorder s)
@@ -9,6 +10,8 @@ val nmst (#s:Type u#s)
          (post:s -> a -> s -> prop)
 : Type u#0
 
+val lift #s #rel #a #pre #post (f:M.mst #s rel a pre post)
+: nmst #s rel a pre post
 
 val return (#s:Type u#s)
            (#rel:preorder s)
@@ -16,11 +19,6 @@ val return (#s:Type u#s)
            (x:a)
 : nmst rel a (fun _ -> True) (fun s0 v s1 -> x == v /\ s0 == s1)
            
-
-let req_t (s:Type) = s -> prop
-let ens_t (s:Type) (a:Type) = s -> a -> s -> prop
-
-
 val bind
       (#s:Type u#s)
       (#a:Type u#a)
@@ -33,11 +31,13 @@ val bind
       (f:nmst rel a req_f ens_f)
       (g:(x:a -> Dv (nmst rel b (req_g x) (ens_g x))))
 : nmst rel b
-  (fun s0 -> req_f s0 /\ (forall x s1. ens_f s0 x s1 ==> (req_g x) s1))
-  (fun s0 r s2 -> req_f s0 /\ (exists x s1. ens_f s0 x s1 /\ (req_g x) s1 /\ (ens_g x) s1 r s2))
+  (fun s0 ->
+    req_f s0 /\
+    (forall x s1. ens_f s0 x s1 ==> (req_g x) s1))
+  (fun s0 r s2 ->
+    req_f s0 /\
+    (exists x s1. ens_f s0 x s1 /\ (req_g x) s1 /\ (ens_g x) s1 r s2))
     
-
-
 val weaken
       (#s:Type u#s)
       (#rel:preorder s)
@@ -47,31 +47,12 @@ val weaken
       (#req_g:req_t s)
       (#ens_g:ens_t s a)
       (f:nmst rel a req_f ens_f)
-    : Pure (nmst rel a req_g ens_g)
-      (requires
-        (forall s. req_g s ==> req_f s) /\
-        (forall s0 x s1. (req_g s0 /\ ens_f s0 x s1) ==> ens_g s0 x s1))
-      (ensures fun _ -> True)
-
+: Pure 
+  (nmst rel a req_g ens_g)
+  (requires
+    (forall s. req_g s ==> req_f s) /\
+    (forall s0 x s1. (req_g s0 /\ ens_f s0 x s1) ==> ens_g s0 x s1))
+  (ensures fun _ -> True)
 
 val flip (#s:Type u#s) (#rel:preorder s) (_:unit)
   : nmst rel bool (fun _ -> True) (fun s0 x s1 -> s0 == s1)
-
-
-val get (#s:Type u#s) (#rel:preorder s) (_:unit)
-  : nmst rel s (fun _ -> True) (fun s0 x s1 -> s0 == s1 /\ x == s0)
-
-
-val put (#s:Type u#s) (#rel:preorder s) (v:s)
-  : nmst rel unit (fun s0 -> rel s0 v /\ True) (fun s0 x s1 -> v == s1)
-
-
-val witnessed (#s:Type u#s) (p: s -> prop) : Type0
-
-
-val witness (#s:Type u#s) (#rel:preorder s) (p: s -> prop { stable p rel })
-  : nmst rel (witnessed p) (fun s0 -> p s0) (fun s0 x s1 -> s0 == s1)
-
-
-val recall (#s:Type u#s) (#rel:preorder s) (p: s -> prop) (w:witnessed p) 
-  : nmst rel unit (fun s0 -> True) (fun s0 x s1 -> s0 == s1 /\ p s1)
